@prefix : <http://purl.dataone.org/odo/SENSO_> .
@prefix dc: <http://purl.org/dc/elements/1.1/> .
@prefix obo: <http://purl.obolibrary.org/obo/> .
@prefix odo: <http://purl.obolibrary.org/odo/> .
@prefix owl: <http://www.w3.org/2002/07/owl#> .
@prefix rdf: <http://www.w3.org/1999/02/22-rdf-syntax-ns#> .
@prefix xml: <http://www.w3.org/XML/1998/namespace> .
@prefix xsd: <http://www.w3.org/2001/XMLSchema#> .
@prefix envo: <http://purl.obolibrary.org/obo/envo#> .
@prefix foaf: <http://xmlns.com/foaf/0.1/> .
@prefix rdfs: <http://www.w3.org/2000/01/rdf-schema#> .
@prefix skos: <http://www.w3.org/2004/02/skos/core#> .
@prefix terms: <http://purl.org/dc/terms/> .
@prefix oboInOwl: <http://www.geneontology.org/formats/oboInOwl#> .
@base <http://purl.dataone.org/odo/SENSO> .

<http://purl.dataone.org/odo/SENSO_> rdf:type owl:Ontology ;
                                     owl:versionIRI <http://purl.dataone.org/odo/SENSO/0.1.0> ;
                                     owl:versionInfo "Version 0.1.0" ;
                                     owl:imports <http://purl.obofoundry.org/obo/DUO.owl> ,
                                                 <http://purl.obofoundry.org/obo/ICO.owl> ;
                                     terms:creator <https://orcid.org/0000-0003-0077-4738> ;
                                     terms:created "2021-09-28"^^xsd:date ;
                                     terms:license <https://creativecommons.org/licenses/by/4.0/> ;
                                     terms:title "Sensitive Data Ontology (SENSO)"@en ;
                                     terms:description "Ontology to support sensitive data annotation of datasets housed at the Arctic Data Center (https://arcticdata.io)"@en .

#################################################################
#    Annotation properties
#################################################################

###  http://purl.obolibrary.org/obo/IAO_0000115
obo:IAO_0000115 rdf:type owl:AnnotationProperty ;
                dc:creator <http://orcid.org/0000-0002-5300-3075> ;
                dc:date "2021-09-28T19:46:54Z"^^xsd:dateTime ;
                rdfs:label "definition"@en .


###  http://purl.obolibrary.org/odo/IAO_0000119
odo:IAO_0000119 rdf:type owl:AnnotationProperty ;
                dc:creator <http://orcid.org/0000-0002-5300-3075> ;
                dc:date "2020-11-04T19:47:37Z"^^xsd:dateTime ;
                rdfs:label "definition source"@en .


###  http://purl.org/dc/elements/1.1/creator
dc:creator rdf:type owl:AnnotationProperty .


###  http://purl.org/dc/elements/1.1/date
dc:date rdf:type owl:AnnotationProperty .


###  http://purl.org/dc/elements/1.1/description
dc:description rdf:type owl:AnnotationProperty .


###  http://www.geneontology.org/formats/oboInOwl#id
oboInOwl:id rdf:type owl:AnnotationProperty .


###  http://www.w3.org/2000/01/rdf-schema#comment
rdfs:comment rdf:type owl:AnnotationProperty .


###  http://www.w3.org/2002/07/owl#sameAs
owl:sameAs rdf:type owl:AnnotationProperty .


###  http://www.w3.org/2004/02/skos/core#altLabel
skos:altLabel rdf:type owl:AnnotationProperty .


#################################################################
#    Object Properties
#################################################################


#################################################################
#    Classes
#################################################################

### http://purl.obolibrary.org/obo/DUO_0000001
obo:DUO_0000001
    obo:IAO_0000115 "A data item that is used to indicate consent permissions for datasets and/or materials, and relates to the purposes for which datasets and/or material might be removed, stored or used."@en ;
    obo:IAO_0000118 "consent code"^^xsd:string ;
    oboInOwl:id "DUO:0000001"^^xsd:string ;
    a owl:Class ;
    rdfs:label "data use permission"@en ;
    rdfs:subClassOf obo:IAO_0000027 .

### http://purl.obolibrary.org/obo/DUO_0000004
obo:DUO_0000004
    obo:IAO_0000115 "This data use permission indicates there is no restriction on use."@en ;
    oboInOwl:id "DUO:0000004"^^xsd:string ;
    oboInOwl:shorthand "NRES"^^xsd:string ;
    a owl:Class ;
    rdfs:comment "20180907, Meeting Moran Melanie: This is to be thought about more carefully - what is the intent when using 'no restriction' as usually users still need to be researchers.", "Note: the NRES alternative term may be confusing as in the UK it also stands for National Research Ethics Service"^^xsd:string ;
    rdfs:label "no restriction"@en ;
    rdfs:subClassOf obo:DUO_0000001 .

### http://purl.obolibrary.org/obo/DUO_0000011
obo:DUO_0000011
    obo:IAO_0000115 "This data use permission indicates that use of the data is limited to the study of population origins or ancestry."@en ;
    obo:IAO_0000118 "population origins/ancestry research"^^xsd:string ;
    oboInOwl:id "DUO:0000011"^^xsd:string ;
    oboInOwl:shorthand "POA"^^xsd:string ;
    a owl:Class ;
    rdfs:label "population origins or ancestry research only"@en ;
    rdfs:subClassOf obo:DUO_0000001 .

### http://purl.obolibrary.org/obo/DUO_0000017
obo:DUO_0000017
    obo:IAO_0000115 "Data use modifiers indicate additional conditions for use."@en ;
    oboInOwl:id "DUO:0000017"^^xsd:string ;
    a owl:Class ;
    rdfs:label "data use modifier"@en ;
    rdfs:subClassOf obo:IAO_0000027 .

### http://purl.obolibrary.org/obo/DUO_0000018
obo:DUO_0000018
    obo:IAO_0000115 "This data use modifier indicates that use of the data is limited to not-for-profit organizations and not-for-profit use, non-commercial use."@en ;
    oboInOwl:id "DUO:0000018"^^xsd:string ;
    oboInOwl:shorthand "NPUNCU"^^xsd:string ;
    a owl:Class ;
    rdfs:label "not for profit, non commercial use only"@en ;
    rdfs:subClassOf obo:DUO_0000017 .

### http://purl.obolibrary.org/obo/DUO_0000019
obo:DUO_0000019
    obo:IAO_0000115 "This data use modifier indicates that requestor agrees to make results of studies using the data available to the larger scientific community."@en ;
    oboInOwl:id "DUO:0000019"^^xsd:string ;
    oboInOwl:shorthand "PUB"^^xsd:string ;
    a owl:Class ;
    rdfs:label "publication required"@en ;
    rdfs:subClassOf obo:DUO_0000017 .

### http://purl.obolibrary.org/obo/DUO_0000020
obo:DUO_0000020
    obo:IAO_0000115 "This data use modifier indicates that the requestor must agree to collaboration with the primary study investigator(s)."@en ;
    oboInOwl:id "DUO:0000020"^^xsd:string ;
    oboInOwl:shorthand "COL"^^xsd:string ;
    a owl:Class ;
    rdfs:comment "This could be coupled with a string describing the primary study investigator(s)."@en ;
    rdfs:label "collaboration required"@en ;
    rdfs:subClassOf obo:DUO_0000017 .

### http://purl.obolibrary.org/obo/DUO_0000021
obo:DUO_0000021
    obo:IAO_0000115 "This data use modifier indicates that the requestor must provide documentation of local IRB/ERB approval."@en ;
    oboInOwl:id "DUO:0000021"^^xsd:string ;
    oboInOwl:shorthand "IRB"^^xsd:string ;
    a owl:Class ;
    rdfs:label "ethics approval required"@en ;
    rdfs:subClassOf obo:DUO_0000017 .

### http://purl.obolibrary.org/obo/DUO_0000026
obo:DUO_0000026
    obo:IAO_0000115 "This data use modifier indicates that use is limited to use by approved users."@en ;
    oboInOwl:id "DUO:0000026"^^xsd:string ;
    oboInOwl:shorthand "US"^^xsd:string ;
    a owl:Class ;
    rdfs:label "user specific restriction"@en ;
    rdfs:subClassOf obo:DUO_0000017 .

### http://purl.obolibrary.org/obo/DUO_0000027
obo:DUO_0000027
    obo:IAO_0000115 "This data use modifier indicates that use is limited to use within an approved project."@en ;
    oboInOwl:id "DUO:0000027"^^xsd:string ;
    oboInOwl:shorthand "PS"^^xsd:string ;
    a owl:Class ;
    rdfs:label "project specific restriction"@en ;
    rdfs:subClassOf obo:DUO_0000017 .

### http://purl.obolibrary.org/obo/DUO_0000028
obo:DUO_0000028
    obo:IAO_0000115 "This data use modifier indicates that use is limited to use within an approved institution."@en ;
    oboInOwl:id "DUO:0000028"^^xsd:string ;
    oboInOwl:shorthand "IS"^^xsd:string ;
    a owl:Class ;
    rdfs:label "institution specific restriction"@en ;
    rdfs:subClassOf obo:DUO_0000017 .

### http://purl.obolibrary.org/obo/DUO_0000042
obo:DUO_0000042
    obo:IAO_0000115 "This data use permission indicates that use is allowed for general research use for any research purpose."@en ;
    oboInOwl:id "DUO:0000042"^^xsd:string ;
    oboInOwl:shorthand "GRU"^^xsd:string ;
    a owl:Class ;
    rdfs:comment "This includes but is not limited to: health/medical/biomedical purposes, fundamental biology research, the study of population origins or ancestry, statistical methods and algorithms development, and social-sciences research."@en ;
    rdfs:label "general research use"@en ;
    rdfs:subClassOf obo:DUO_0000001 .

### http://purl.obolibrary.org/obo/DUO_0000043
obo:DUO_0000043
    obo:IAO_0000115 "This data use modifier indicates that use is allowed for clinical use and care."@en ;
    oboInOwl:id "DUO:0000043"^^xsd:string ;
    oboInOwl:shorthand "CC"^^xsd:string ;
    a owl:Class ;
    rdfs:comment "Clinical Care is defined as Health care or services provided at home, in a healthcare facility or hospital. Data may be used for clinical decision making."@en ;
    rdfs:label "clinical care use"@en ;
    rdfs:subClassOf obo:DUO_0000017 .

### http://purl.obolibrary.org/obo/DUO_0000045
obo:DUO_0000045
    obo:IAO_0000115 "This data use modifier indicates that use of the data is limited to not-for-profit organizations."@en ;
    oboInOwl:id "DUO:0000045"^^xsd:string ;
    oboInOwl:shorthand "NPU"^^xsd:string ;
    a owl:Class ;
    rdfs:label "not for profit organisation use only"@en ;
    rdfs:subClassOf obo:DUO_0000018 .

### http://purl.obolibrary.org/obo/DUO_0000046
obo:DUO_0000046
    obo:IAO_0000115 "This data use modifier indicates that use of the data is limited to not-for-profit use."@en ;
    oboInOwl:id "DUO:0000046"^^xsd:string ;
    oboInOwl:shorthand "NCU"^^xsd:string ;
    a owl:Class ;
    rdfs:comment "This indicates that data can be used by commercial organisations for research purposes, but not commercial purposes."@en ;
    rdfs:label "non-commercial use only"@en ;
    rdfs:subClassOf obo:DUO_0000018 .

###  http://purl.dataone.org/odo/SENSO_00000001
odo:SENSO_00000001 
    rdf:type owl:Class ;
    obo:IAO_0000115 "Data sensitivity categories assign a level of sensitivity for datasets and provide guidelines for acceptable distribution and use." ;
    dc:creator <http://orcid.org/0000-0003-0077-4738> ;
    dc:date "2021-09-28"^^xsd:date ;
    rdfs:label "Data Sensitivity Category"@en .

###  http://purl.dataone.org/odo/SENSO_00000002
odo:SENSO_00000002
    rdf:type owl:Class ;
    obo:IAO_0000115 "Non-sensitive data"@en ;
    dc:creator <http://orcid.org/0000-0003-0077-4738> ;
    dc:date "2021-09-28"^^xsd:date ;
    dc:description "None of the data includes sensitive or protected information."@en ;
    rdfs:label "Non-sensitive data"@en ;
    rdfs:subClassOf odo:SENSO_00000001 .

###  http://purl.dataone.org/odo/SENSO_00000003
odo:SENSO_00000003
    rdf:type owl:Class ;
    obo:IAO_0000115 "Some or all data is sensitive but has been made safe for open distribution"@en ;
    dc:creator <http://orcid.org/0000-0003-0077-4738> ;
    dc:date "2021-09-28"^^xsd:date ;
    dc:description "Sensitive data has been de-identified, anonymized, aggregated, or summarized to remove sensitivities and enable safe data distribution. Examples include ensuring that human subjects data, protected species data, archaeological site locations and personally identifiable information have been properly anonymized, aggregated and summarized."@en ;
    rdfs:label "De-identified data"@en ;
    rdfs:subClassOf odo:SENSO_00000001 .

###  http://purl.dataone.org/odo/SENSO_00000004
odo:SENSO_00000004
    rdf:type owl:Class ;
    obo:IAO_0000115 "Some or all data is sensitive and should not be distributed"@en ;
    dc:creator <http://orcid.org/0000-0003-0077-4738> ;
    dc:date "2021-09-28"^^xsd:date ;
    dc:description "The data contains human subjects data or other sensitive data. Release of the data could cause harm or violate statutes, and must remain confidential following restrictions from an Institutional Review Board (IRB) or similar body."@en ;
    rdfs:label "Sensitive data"@en ;
    rdfs:subClassOf odo:SENSO_00000001 .
