@prefix : <http://purl.dataone.org/odo/SENSO_> .
@prefix dc: <http://purl.org/dc/elements/1.1/> .
@prefix obo: <http://purl.obolibrary.org/obo/> .
@prefix odo: <http://purl.obolibrary.org/odo/> .
@prefix owl: <http://www.w3.org/2002/07/owl#> .
@prefix rdf: <http://www.w3.org/1999/02/22-rdf-syntax-ns#> .
@prefix xml: <http://www.w3.org/XML/1998/namespace> .
@prefix xsd: <http://www.w3.org/2001/XMLSchema#> .
@prefix envo: <http://purl.obolibrary.org/obo/envo#> .
@prefix foaf: <http://xmlns.com/foaf/0.1/> .
@prefix rdfs: <http://www.w3.org/2000/01/rdf-schema#> .
@prefix skos: <http://www.w3.org/2004/02/skos/core#> .
@prefix terms: <http://purl.org/dc/terms/> .
@prefix oboInOwl: <http://www.geneontology.org/formats/oboInOwl#> .
@base <http://purl.dataone.org/odo/SENSO_> .

<http://purl.dataone.org/odo/SENSO_> rdf:type owl:Ontology ;
                                      owl:versionIRI <http://purl.dataone.org/odo/SENSO/0.1.0> ;
                                      owl:imports <http://purl.obofoundry.org/obo/DUO.owl> ;
                                      terms:created "2021-09-28"^^xsd:date ;
                                      terms:creator <https://orcid.org/0000-0003-0077-4738> ;
                                      terms:description "Ontology to support sensitive data annotation of datasets housed at the Arctic Data Center (https://arcticdata.io)"@en ;
                                      terms:license <https://creativecommons.org/licenses/by/4.0/> ;
                                      terms:title "Sensitive Data Ontology (SENSO)"@en ;
                                      owl:versionInfo "Version 0.1.0" .

#################################################################
#    Annotation properties
#################################################################

###  http://purl.obolibrary.org/obo/IAO_0000115
obo:IAO_0000115 rdf:type owl:AnnotationProperty ;
                dc:creator <http://orcid.org/0000-0002-5300-3075> ;
                dc:date "2021-09-28T19:46:54Z"^^xsd:dateTime ;
                rdfs:label "definition"@en .


###  http://purl.obolibrary.org/obo/IAO_0000118
obo:IAO_0000118 rdf:type owl:AnnotationProperty .


###  http://purl.obolibrary.org/odo/IAO_0000119
odo:IAO_0000119 rdf:type owl:AnnotationProperty ;
                dc:creator <http://orcid.org/0000-0002-5300-3075> ;
                dc:date "2020-11-04T19:47:37Z"^^xsd:dateTime ;
                rdfs:label "definition source"@en .


###  http://purl.org/dc/elements/1.1/creator
dc:creator rdf:type owl:AnnotationProperty .


###  http://purl.org/dc/elements/1.1/date
dc:date rdf:type owl:AnnotationProperty .


###  http://purl.org/dc/elements/1.1/description
dc:description rdf:type owl:AnnotationProperty .


###  http://purl.org/dc/terms/created
terms:created rdf:type owl:AnnotationProperty .


###  http://purl.org/dc/terms/creator
terms:creator rdf:type owl:AnnotationProperty .


###  http://purl.org/dc/terms/description
terms:description rdf:type owl:AnnotationProperty .


###  http://purl.org/dc/terms/license
terms:license rdf:type owl:AnnotationProperty .


###  http://purl.org/dc/terms/title
terms:title rdf:type owl:AnnotationProperty .


###  http://www.geneontology.org/formats/oboInOwl#id
oboInOwl:id rdf:type owl:AnnotationProperty .


###  http://www.geneontology.org/formats/oboInOwl#shorthand
oboInOwl:shorthand rdf:type owl:AnnotationProperty .


###  http://www.w3.org/2000/01/rdf-schema#comment
rdfs:comment rdf:type owl:AnnotationProperty .


###  http://www.w3.org/2002/07/owl#sameAs
owl:sameAs rdf:type owl:AnnotationProperty .


###  http://www.w3.org/2004/02/skos/core#altLabel
skos:altLabel rdf:type owl:AnnotationProperty .


#################################################################
#    Datatypes
#################################################################

###  http://www.w3.org/2001/XMLSchema#date
xsd:date rdf:type rdfs:Datatype .


#################################################################
#    Classes
#################################################################

###  http://purl.obolibrary.org/obo/DUO_0000001
obo:DUO_0000001 rdf:type owl:Class ;
                rdfs:subClassOf obo:IAO_0000027 ;
                obo:IAO_0000115 "A data item that is used to indicate consent permissions for datasets and/or materials, and relates to the purposes for which datasets and/or material might be removed, stored or used."@en ;
                obo:IAO_0000118 "consent code"^^xsd:string ;
                oboInOwl:id "DUO:0000001"^^xsd:string ;
                rdfs:label "data use permission"@en .


###  http://purl.obolibrary.org/obo/DUO_0000004
obo:DUO_0000004 rdf:type owl:Class ;
                rdfs:subClassOf obo:DUO_0000001 ;
                obo:IAO_0000115 "This data use permission indicates there is no restriction on use."@en ;
                oboInOwl:id "DUO:0000004"^^xsd:string ;
                oboInOwl:shorthand "NRES"^^xsd:string ;
                rdfs:comment "20180907, Meeting Moran Melanie: This is to be thought about more carefully - what is the intent when using 'no restriction' as usually users still need to be researchers." ,
                             "Note: the NRES alternative term may be confusing as in the UK it also stands for National Research Ethics Service"^^xsd:string ;
                rdfs:label "no restriction"@en .


###  http://purl.obolibrary.org/obo/DUO_0000011
obo:DUO_0000011 rdf:type owl:Class ;
                rdfs:subClassOf obo:DUO_0000001 ;
                obo:IAO_0000115 "This data use permission indicates that use of the data is limited to the study of population origins or ancestry."@en ;
                obo:IAO_0000118 "population origins/ancestry research"^^xsd:string ;
                oboInOwl:id "DUO:0000011"^^xsd:string ;
                oboInOwl:shorthand "POA"^^xsd:string ;
                rdfs:label "population origins or ancestry research only"@en .


###  http://purl.obolibrary.org/obo/DUO_0000017
obo:DUO_0000017 rdf:type owl:Class ;
                rdfs:subClassOf obo:IAO_0000027 ;
                obo:IAO_0000115 "Data use modifiers indicate additional conditions for use."@en ;
                oboInOwl:id "DUO:0000017"^^xsd:string ;
                rdfs:label "data use modifier"@en .


###  http://purl.obolibrary.org/obo/DUO_0000018
obo:DUO_0000018 rdf:type owl:Class ;
                rdfs:subClassOf obo:DUO_0000017 ;
                obo:IAO_0000115 "This data use modifier indicates that use of the data is limited to not-for-profit organizations and not-for-profit use, non-commercial use."@en ;
                oboInOwl:id "DUO:0000018"^^xsd:string ;
                oboInOwl:shorthand "NPUNCU"^^xsd:string ;
                rdfs:label "not for profit, non commercial use only"@en .


###  http://purl.obolibrary.org/obo/DUO_0000019
obo:DUO_0000019 rdf:type owl:Class ;
                rdfs:subClassOf obo:DUO_0000017 ;
                obo:IAO_0000115 "This data use modifier indicates that requestor agrees to make results of studies using the data available to the larger scientific community."@en ;
                oboInOwl:id "DUO:0000019"^^xsd:string ;
                oboInOwl:shorthand "PUB"^^xsd:string ;
                rdfs:label "publication required"@en .


###  http://purl.obolibrary.org/obo/DUO_0000020
obo:DUO_0000020 rdf:type owl:Class ;
                rdfs:subClassOf obo:DUO_0000017 ;
                obo:IAO_0000115 "This data use modifier indicates that the requestor must agree to collaboration with the primary study investigator(s)."@en ;
                oboInOwl:id "DUO:0000020"^^xsd:string ;
                oboInOwl:shorthand "COL"^^xsd:string ;
                rdfs:comment "This could be coupled with a string describing the primary study investigator(s)."@en ;
                rdfs:label "collaboration required"@en .


###  http://purl.obolibrary.org/obo/DUO_0000021
obo:DUO_0000021 rdf:type owl:Class ;
                rdfs:subClassOf obo:DUO_0000017 ;
                obo:IAO_0000115 "This data use modifier indicates that the requestor must provide documentation of local IRB/ERB approval."@en ;
                oboInOwl:id "DUO:0000021"^^xsd:string ;
                oboInOwl:shorthand "IRB"^^xsd:string ;
                rdfs:label "ethics approval required"@en .


###  http://purl.obolibrary.org/obo/DUO_0000026
obo:DUO_0000026 rdf:type owl:Class ;
                rdfs:subClassOf obo:DUO_0000017 ;
                obo:IAO_0000115 "This data use modifier indicates that use is limited to use by approved users."@en ;
                oboInOwl:id "DUO:0000026"^^xsd:string ;
                oboInOwl:shorthand "US"^^xsd:string ;
                rdfs:label "user specific restriction"@en .


###  http://purl.obolibrary.org/obo/DUO_0000027
obo:DUO_0000027 rdf:type owl:Class ;
                rdfs:subClassOf obo:DUO_0000017 ;
                obo:IAO_0000115 "This data use modifier indicates that use is limited to use within an approved project."@en ;
                oboInOwl:id "DUO:0000027"^^xsd:string ;
                oboInOwl:shorthand "PS"^^xsd:string ;
                rdfs:label "project specific restriction"@en .


###  http://purl.obolibrary.org/obo/DUO_0000028
obo:DUO_0000028 rdf:type owl:Class ;
                rdfs:subClassOf obo:DUO_0000017 ;
                obo:IAO_0000115 "This data use modifier indicates that use is limited to use within an approved institution."@en ;
                oboInOwl:id "DUO:0000028"^^xsd:string ;
                oboInOwl:shorthand "IS"^^xsd:string ;
                rdfs:label "institution specific restriction"@en .


###  http://purl.obolibrary.org/obo/DUO_0000042
obo:DUO_0000042 rdf:type owl:Class ;
                rdfs:subClassOf obo:DUO_0000001 ;
                obo:IAO_0000115 "This data use permission indicates that use is allowed for general research use for any research purpose."@en ;
                oboInOwl:id "DUO:0000042"^^xsd:string ;
                oboInOwl:shorthand "GRU"^^xsd:string ;
                rdfs:comment "This includes but is not limited to: health/medical/biomedical purposes, fundamental biology research, the study of population origins or ancestry, statistical methods and algorithms development, and social-sciences research."@en ;
                rdfs:label "general research use"@en .


###  http://purl.obolibrary.org/obo/DUO_0000043
obo:DUO_0000043 rdf:type owl:Class ;
                rdfs:subClassOf obo:DUO_0000017 ;
                obo:IAO_0000115 "This data use modifier indicates that use is allowed for clinical use and care."@en ;
                oboInOwl:id "DUO:0000043"^^xsd:string ;
                oboInOwl:shorthand "CC"^^xsd:string ;
                rdfs:comment "Clinical Care is defined as Health care or services provided at home, in a healthcare facility or hospital. Data may be used for clinical decision making."@en ;
                rdfs:label "clinical care use"@en .


###  http://purl.obolibrary.org/obo/DUO_0000045
obo:DUO_0000045 rdf:type owl:Class ;
                rdfs:subClassOf obo:DUO_0000018 ;
                obo:IAO_0000115 "This data use modifier indicates that use of the data is limited to not-for-profit organizations."@en ;
                oboInOwl:id "DUO:0000045"^^xsd:string ;
                oboInOwl:shorthand "NPU"^^xsd:string ;
                rdfs:label "not for profit organisation use only"@en .


###  http://purl.obolibrary.org/obo/DUO_0000046
obo:DUO_0000046 rdf:type owl:Class ;
                rdfs:subClassOf obo:DUO_0000018 ;
                obo:IAO_0000115 "This data use modifier indicates that use of the data is limited to not-for-profit use."@en ;
                oboInOwl:id "DUO:0000046"^^xsd:string ;
                oboInOwl:shorthand "NCU"^^xsd:string ;
                rdfs:comment "This indicates that data can be used by commercial organisations for research purposes, but not commercial purposes."@en ;
                rdfs:label "non-commercial use only"@en .


###  http://purl.obolibrary.org/obo/IAO_0000027
obo:IAO_0000027 rdf:type owl:Class ;
    obo:IAO_0000115 "An information content entity that is intended to be a truthful statement about something (modulo, e.g., measurement precision or other systematic errors) and is constructed/acquired by a method which reliably tends to produce (approximately) truthful statements."@en ;
    oboInOwl:id "IAO:0000027"^^xsd:string ;
    rdfs:label "data item"@en .


###  http://purl.obolibrary.org/odo/SENSO_00000001
odo:SENSO_00000001 rdf:type owl:Class ;
                   obo:IAO_0000115 "Data sensitivity categories assign a level of sensitivity for datasets and provide guidelines for acceptable distribution and use." ;
                   dc:creator <http://orcid.org/0000-0003-0077-4738> ;
                   dc:date "2021-09-28"^^xsd:date ;
                   rdfs:label "Data Sensitivity Category"@en .


###  http://purl.obolibrary.org/odo/SENSO_00000002
odo:SENSO_00000002 rdf:type owl:Class ;
                   rdfs:subClassOf odo:SENSO_00000001 ;
                   obo:IAO_0000115 "Non-sensitive data"@en ;
                   dc:creator <http://orcid.org/0000-0003-0077-4738> ;
                   dc:date "2021-09-28"^^xsd:date ;
                   dc:description "None of the data includes sensitive or protected information."@en ;
                   rdfs:label "Non-sensitive data"@en ;
                   owl:sameAs odo:SENSO_00000006 .


###  http://purl.obolibrary.org/odo/SENSO_00000003
odo:SENSO_00000003 rdf:type owl:Class ;
                   rdfs:subClassOf odo:SENSO_00000001 ;
                   obo:IAO_0000115 "Some or all data is sensitive but has been made safe for open distribution"@en ;
                   dc:creator <http://orcid.org/0000-0003-0077-4738> ;
                   dc:date "2021-09-28"^^xsd:date ;
                   dc:description "Sensitive data has been de-identified, anonymized, aggregated, or summarized to remove sensitivities and enable safe data distribution. Examples include ensuring that human subjects data, protected species data, archaeological site locations and personally identifiable information have been properly anonymized, aggregated and summarized."@en ;
                   rdfs:label "De-identified data"@en ;
                   owl:sameAs odo:SENSO_00000007 .


###  http://purl.obolibrary.org/odo/SENSO_00000004
odo:SENSO_00000004 rdf:type owl:Class ;
                   rdfs:subClassOf odo:SENSO_00000001 ;
                   obo:IAO_0000115 "Some or all data is sensitive and should not be distributed"@en ;
                   dc:creator <http://orcid.org/0000-0003-0077-4738> ;
                   dc:date "2021-09-28"^^xsd:date ;
                   dc:description "The data contains human subjects data or other sensitive data. Release of the data could cause harm or violate statutes, and must remain confidential following restrictions from an Institutional Review Board (IRB) or similar body."@en ;
                   rdfs:label "Sensitive data"@en .


###  http://purl.obolibrary.org/odo/SENSO_00000005
odo:SENSO_00000005 rdf:type owl:Class ;
                   rdfs:subClassOf odo:SENSO_00000001 ;
                   dc:creator <http://orcid.org/0000-0003-0077-4738> ;
                   dc:date "2021-09-28"^^xsd:date ;
                   obo:IAO_0000115 "The DataTags sensitive data categories"@en ;
                   dc:description "The DataTags categories enable classification of data along an axis of sensitivity or confidentiality ranging from completely non-confidential to highly sensitive. Each DataTag is referred to with a color. The system was created through the Harvard IQSS DataTags project (https://datatags.org).."@en ;
                   rdfs:label "DataTag" .


###  http://purl.obolibrary.org/odo/SENSO_00000006
odo:SENSO_00000006 rdf:type owl:Class ;
                   rdfs:subClassOf odo:SENSO_00000005 ;
                   dc:creator <http://orcid.org/0000-0003-0077-4738> ;
                   dc:date "2021-09-28"^^xsd:date ;
                   obo:IAO_0000115 "Non-confidential information"@en ;
                   rdfs:label "DataTag Blue" .


###  http://purl.obolibrary.org/odo/SENSO_00000007
odo:SENSO_00000007 rdf:type owl:Class ;
                   rdfs:subClassOf odo:SENSO_00000005 ;
                   dc:creator <http://orcid.org/0000-0003-0077-4738> ;
                   dc:date "2021-09-28"^^xsd:date ;
                   obo:IAO_0000115 "Non-confidential information"@en ;
                   rdfs:label "DataTag Green" .


###  http://purl.obolibrary.org/odo/SENSO_00000008
odo:SENSO_00000008 rdf:type owl:Class ;
                   rdfs:subClassOf odo:SENSO_00000005 ;
                   dc:creator <http://orcid.org/0000-0003-0077-4738> ;
                   dc:date "2021-09-28"^^xsd:date ;
                   obo:IAO_0000115 "Potentially harmful personal information"@en ;
                   rdfs:label "DataTag Yellow" .


###  http://purl.obolibrary.org/odo/SENSO_00000009
odo:SENSO_00000009 rdf:type owl:Class ;
                   rdfs:subClassOf odo:SENSO_00000005 ;
                   dc:creator <http://orcid.org/0000-0003-0077-4738> ;
                   dc:date "2021-09-28"^^xsd:date ;
                   obo:IAO_0000115 "Sensitive personal information"@en ;
                   rdfs:label "DataTag Orange" .


###  http://purl.obolibrary.org/odo/SENSO_00000010
odo:SENSO_00000010 rdf:type owl:Class ;
                   rdfs:subClassOf odo:SENSO_00000005 ;
                   dc:creator <http://orcid.org/0000-0003-0077-4738> ;
                   dc:date "2021-09-28"^^xsd:date ;
                   obo:IAO_0000115 "Very sensitive personal information"@en ;
                   rdfs:label "DataTag Red" .


###  http://purl.obolibrary.org/odo/SENSO_00000011
odo:SENSO_00000011 rdf:type owl:Class ;
                   rdfs:subClassOf odo:SENSO_00000005 ;
                   dc:creator <http://orcid.org/0000-0003-0077-4738> ;
                   dc:date "2021-09-28"^^xsd:date ;
                   obo:IAO_0000115 "Maximum sensitive personal information"@en ;
                   rdfs:label "DataTag Crimson" .


###  Generated by the OWL API (version 4.5.9.2019-02-01T07:24:44Z) https://github.com/owlcs/owlapi
