<?xml version="1.0"?>
<rdf:RDF xmlns="http://purl.dataone.org/odo/ecso.owl#"
     xml:base="http://purl.dataone.org/odo/ecso.owl"
     xmlns:owl="http://www.w3.org/2002/07/owl#"
     xmlns:oboInOwl="http://www.geneontology.org/formats/oboInOwl#"
     xmlns:ns="http://creativecommons.org/ns#"
     xmlns:xsd="http://www.w3.org/2001/XMLSchema#"
     xmlns:skos="http://www.w3.org/2004/02/skos/core#"
     xmlns:rdfs="http://www.w3.org/2000/01/rdf-schema#"
     xmlns:rdf="http://www.w3.org/1999/02/22-rdf-syntax-ns#"
     xmlns:ecso="http://purl.dataone.org/odo/2/ecso.owl#"
     xmlns:xml="http://www.w3.org/XML/1998/namespace"
     xmlns:oboe-core="http://ecoinformatics.org/oboe/oboe.1.2/oboe-core.owl#"
     xmlns:odo="http://purl.dataone.org/odo/"
     xmlns:obo="http://purl.obolibrary.org/obo/"
     xmlns:dc="http://purl.org/dc/elements/1.1/">
    <owl:Ontology rdf:about="http://purl.dataone.org/odo/ecso.owl">
        <owl:versionIRI rdf:resource="http://purl.dataone.org/odo/2/ecso.owl"/>
        <owl:imports rdf:resource="http://purl.dataone.org/odo/ECSO_"/>
        <owl:imports rdf:resource="http://www.semanticweb.org/elizabetholson/ontologies/2017/5/untitled-ontology-14"/>
    </owl:Ontology>
    


    <!-- 
    ///////////////////////////////////////////////////////////////////////////////////////
    //
    // Annotation properties
    //
    ///////////////////////////////////////////////////////////////////////////////////////
     -->

    


    <!-- http://purl.org/dc/elements/1.1/creator -->

    <owl:AnnotationProperty rdf:about="http://purl.org/dc/elements/1.1/creator"/>
    


    <!-- 
    ///////////////////////////////////////////////////////////////////////////////////////
    //
    // Object Properties
    //
    ///////////////////////////////////////////////////////////////////////////////////////
     -->

    


    <!-- http://www.semanticweb.org/elizabetholson/ontologies/2017/5/untitled-ontology-14#ECSO_00000000000000005017 -->

    <rdf:Description rdf:about="http://www.semanticweb.org/elizabetholson/ontologies/2017/5/untitled-ontology-14#ECSO_00000000000000005017">
        <rdfs:domain rdf:resource="http://purl.dataone.org/odo/ECSO_00000010"/>
        <rdfs:domain rdf:resource="http://purl.dataone.org/odo/ECSO_00000025"/>
        <rdfs:range rdf:resource="http://purl.dataone.org/odo/ECSO_00000546"/>
    </rdf:Description>
    


    <!-- http://www.semanticweb.org/elizabetholson/ontologies/2017/5/untitled-ontology-14#ECSO_00000000000000005018 -->

    <rdf:Description rdf:about="http://www.semanticweb.org/elizabetholson/ontologies/2017/5/untitled-ontology-14#ECSO_00000000000000005018">
        <rdfs:domain rdf:resource="http://purl.dataone.org/odo/ECSO_00000025"/>
        <rdfs:range rdf:resource="http://purl.dataone.org/odo/ECSO_00000010"/>
    </rdf:Description>
    


    <!-- http://www.semanticweb.org/elizabetholson/ontologies/2017/5/untitled-ontology-14#ECSO_00000000000000005019 -->

    <rdf:Description rdf:about="http://www.semanticweb.org/elizabetholson/ontologies/2017/5/untitled-ontology-14#ECSO_00000000000000005019">
        <rdfs:domain rdf:resource="http://purl.dataone.org/odo/ECSO_00000010"/>
        <rdfs:range rdf:resource="http://purl.dataone.org/odo/ECSO_00000025"/>
    </rdf:Description>
    


    <!-- 
    ///////////////////////////////////////////////////////////////////////////////////////
    //
    // Classes
    //
    ///////////////////////////////////////////////////////////////////////////////////////
     -->

    


    <!-- http://purl.dataone.org/odo/ECSO_00000035 -->

    <rdf:Description rdf:about="http://purl.dataone.org/odo/ECSO_00000035">
        <rdfs:subClassOf>
            <owl:Restriction>
                <owl:onProperty rdf:resource="http://purl.obolibrary.org/obo/RO_0002473"/>
                <owl:qualifiedCardinality rdf:datatype="http://www.w3.org/2001/XMLSchema#nonNegativeInteger">1</owl:qualifiedCardinality>
                <owl:onClass rdf:resource="http://purl.dataone.org/odo/ECSO_00000571"/>
            </owl:Restriction>
        </rdfs:subClassOf>
        <odo:ECSO_01000001>Elizabeth Olson, http://orcid.org/0000-0001-8622-9698</odo:ECSO_01000001>
        <odo:ECSO_01000003>https://serc.carleton.edu/microbelife/research_methods/biogeochemical/organic_carbon.html</odo:ECSO_01000003>
        <skos:definition>A system that has the capacity to store or release carbon, in the form of the organic matter that is able to pass through a filter (filters generally range in size between 0.7 and 0.22 um)</skos:definition>
    </rdf:Description>
    


    <!-- http://purl.dataone.org/odo/ECSO_00000206 -->

    <rdf:Description rdf:about="http://purl.dataone.org/odo/ECSO_00000206">
        <owl:disjointWith rdf:resource="http://purl.dataone.org/odo/ECSO_00000336"/>
        <odo:ECSO_01000001>Elizabeth Olson, http://orcid.org/0000-0001-8622-9698</odo:ECSO_01000001>
        <odo:ECSO_01000003>http://www.dictionary.com/browse/carbon-fixation</odo:ECSO_01000003>
        <skos:definition>A system that has the capacity to store or release carbon that was originally atmospheric carbon dioxide that has been converted into organic carbon compounds, usually by plants and algae via photosynthesis</skos:definition>
    </rdf:Description>
    


    <!-- http://purl.dataone.org/odo/ECSO_00000331 -->

    <rdf:Description rdf:about="http://purl.dataone.org/odo/ECSO_00000331">
        <owl:disjointWith rdf:resource="http://purl.dataone.org/odo/ECSO_00000341"/>
        <odo:ECSO_01000001>Elizabeth Olson, http://orcid.org/0000-0001-8622-9698</odo:ECSO_01000001>
        <odo:ECSO_01000003>https://en.wikipedia.org/wiki/Total_organic_carbon
and
https://en.wikipedia.org/wiki/Organic_compound</odo:ECSO_01000003>
        <skos:definition>A system that has the capacity to store or release carbon that is either of a biologic origin or can be found or incorporated into a living organism.</skos:definition>
    </rdf:Description>
    


    <!-- http://purl.dataone.org/odo/ECSO_00000336 -->

    <rdf:Description rdf:about="http://purl.dataone.org/odo/ECSO_00000336">
        <odo:ECSO_01000001>Elizabeth Olson, http://orcid.org/0000-0001-8622-9698</odo:ECSO_01000001>
        <odo:ECSO_01000003>http://soilquality.org.au/factsheets/organic-carbon-pools</odo:ECSO_01000003>
        <odo:ECSO_01000004>Particulate organic carbon also decomposes relatively quickly (years to decades) and provides an important source of energy for soil microorganisms. It also plays an important role in maintaining soil structure and providing soil nutrients. Plant residues and particulate organic carbon are often referred to as ‘labile carbon’ because they cycle in the soil relatively quickly.</odo:ECSO_01000004>
        <odo:ECSO_01000005>http://soilquality.org.au/factsheets/organic-carbon-pools</odo:ECSO_01000005>
        <skos:definition>A system that has the capacity to store or release carbon, in the form of pieces of plant debris 0.053–2 mm in size.</skos:definition>
    </rdf:Description>
    


    <!-- http://purl.dataone.org/odo/ECSO_00000341 -->

    <rdf:Description rdf:about="http://purl.dataone.org/odo/ECSO_00000341"/>
    


    <!-- http://purl.dataone.org/odo/ECSO_00000504 -->

    <rdf:Description rdf:about="http://purl.dataone.org/odo/ECSO_00000504">
        <rdfs:subClassOf>
            <owl:Restriction>
                <owl:onProperty rdf:resource="http://purl.obolibrary.org/obo/BFO_0000050"/>
                <owl:someValuesFrom rdf:resource="http://www.purl.dataone.org/odo#ECSO_0000010050"/>
            </owl:Restriction>
        </rdfs:subClassOf>
    </rdf:Description>
    


    <!-- http://purl.dataone.org/odo/ECSO_00000546 -->

    <rdf:Description rdf:about="http://purl.dataone.org/odo/ECSO_00000546">
        <rdfs:subClassOf rdf:resource="http://ecoinformatics.org/oboe/oboe.1.2/oboe-core.owl#OWLClassImpl_67f86d37_7782_477b_9509_4532fd0caa86"/>
        <rdfs:subClassOf rdf:resource="http://purl.obolibrary.org/obo/BFO_0000003"/>
    </rdf:Description>
    


    <!-- http://purl.obolibrary.org/obo/ENVO_01000155 -->

    <rdf:Description rdf:about="http://purl.obolibrary.org/obo/ENVO_01000155">
        <oboInOwl:hasExactSynonym>organic matter</oboInOwl:hasExactSynonym>
    </rdf:Description>
    


    <!-- http://purl.obolibrary.org/obo/RO_0000056#carbon_cycling -->

    <rdf:Description rdf:about="http://purl.obolibrary.org/obo/RO_0000056#carbon_cycling">
        <rdfs:subClassOf>
            <owl:Restriction>
                <owl:onProperty rdf:resource="http://www.w3.org/TR/skos-reference/skos-owl1-dl#OWLObjectPropertyImpl_55588ab6_d047_45f5_b8b1_006a8ddd8fd4"/>
                <owl:someValuesFrom rdf:resource="http://purl.dataone.org/odo/ECSO_00000010"/>
            </owl:Restriction>
        </rdfs:subClassOf>
    </rdf:Description>
    


    <!-- http://www.purl.dataone.org/odo#ECSO_0000010050 -->

    <owl:Class rdf:about="http://www.purl.dataone.org/odo#ECSO_0000010050">
        <rdfs:subClassOf rdf:resource="http://purl.obolibrary.org/obo/ENVO_01000155"/>
        <odo:ECSO_01000001>Elizabeth Olson, https://orcid.org/0000-0001-8622-9698</odo:ECSO_01000001>
        <odo:ECSO_01000003>http://www.ozcoasts.gov.au/indicators/sediment_org_matter.jsp</odo:ECSO_01000003>
        <dc:creator rdf:datatype="http://www.w3.org/2001/XMLSchema#string">Elizabeth Olson</dc:creator>
        <rdfs:label xml:lang="en">labile organic material</rdfs:label>
        <skos:definition>organic matter with low TOC:TN ratios (e.g. phytoplankton) that breaks down easily</skos:definition>
    </owl:Class>
    


    <!-- http://www.purl.dataone.org/odo#ECSO_0000010051 -->

    <owl:Class rdf:about="http://www.purl.dataone.org/odo#ECSO_0000010051">
        <rdfs:subClassOf rdf:resource="http://purl.obolibrary.org/obo/ENVO_01000155"/>
        <odo:ECSO_01000001>Elizabeth Olson, http://orcid.org/0000-0001-8622-9698</odo:ECSO_01000001>
        <odo:ECSO_01000003>http://www.ozcoasts.gov.au/indicators/sediment_org_matter.jsp</odo:ECSO_01000003>
        <dc:creator rdf:datatype="http://www.w3.org/2001/XMLSchema#string">Elizabeth Olson</dc:creator>
        <rdfs:label xml:lang="en">refactory organic material</rdfs:label>
        <skos:definition>organic compounds (woody debris made of lignin and cellulose) have very high TOC:TN ratios and are highly resistant to degradation</skos:definition>
    </owl:Class>
    


    <!-- http://www.purl.dataone.org/odo#ECSO_0000010052 -->

    <owl:Class rdf:about="http://www.purl.dataone.org/odo#ECSO_0000010052">
        <rdfs:subClassOf rdf:resource="http://purl.dataone.org/odo/ECSO_00000206"/>
        <odo:ECSO_01000001>Elizabeth Olson, http://orcid.org/0000-0001-8622-9698</odo:ECSO_01000001>
        <odo:ECSO_01000003>https://en.wikipedia.org/wiki/Death</odo:ECSO_01000003>
        <dc:creator rdf:datatype="http://www.w3.org/2001/XMLSchema#string">Elizabeth Olson</dc:creator>
        <dc:date rdf:datatype="http://www.w3.org/2001/XMLSchema#dateTime">2017-06-30T16:39:55Z</dc:date>
        <rdfs:label xml:lang="en">Total Non-Living Biomass Carbon Pool</rdfs:label>
        <skos:definition>A system that has the capacity to store or release carbon, via processes inherient to the condition of death (the cessation of all biological functions that sustain a living organism).</skos:definition>
    </owl:Class>
    


    <!-- 
    ///////////////////////////////////////////////////////////////////////////////////////
    //
    // Annotations
    //
    ///////////////////////////////////////////////////////////////////////////////////////
     -->

    <rdf:Description rdf:about="http://purl.dataone.org/odo/ECSO_00000034">
        <odo:ECSO_01000001>Elizabeth Olson, http://orcid.org/0000-0001-8622-9698</odo:ECSO_01000001>
    </rdf:Description>
    <rdf:Description rdf:about="http://purl.dataone.org/odo/ECSO_00000343">
        <odo:ECSO_01000001>Elizabeth Olson, http://orcid.org/0000-0001-8622-9698</odo:ECSO_01000001>
        <odo:ECSO_01000003>https://en.wikipedia.org/wiki/Life</odo:ECSO_01000003>
        <skos:definition>A system that has the capacity to store or release carbon, via processes inherient to the condition of life (an organism maintianing homeostasis, composed of cells, undergo metabolism, can grow, adapt to their enviornment, respond to stimuli and reproduce).</skos:definition>
    </rdf:Description>
    <rdf:Description rdf:about="www.purl.dataone.org/odo/ECSO_00010000">
        <skos:hiddenLabel>odo:Ecosystem</skos:hiddenLabel>
    </rdf:Description>
    


    <!-- 
    ///////////////////////////////////////////////////////////////////////////////////////
    //
    // General axioms
    //
    ///////////////////////////////////////////////////////////////////////////////////////
     -->

    <rdf:Description>
        <rdf:type rdf:resource="http://www.w3.org/2002/07/owl#AllDisjointClasses"/>
        <owl:members rdf:parseType="Collection">
            <rdf:Description rdf:about="http://purl.obolibrary.org/obo/ENVO_01000786"/>
            <rdf:Description rdf:about="http://purl.obolibrary.org/obo/ENVO_01000793"/>
            <rdf:Description rdf:about="http://purl.obolibrary.org/obo/ENVO_01000830"/>
            <rdf:Description rdf:about="http://purl.obolibrary.org/obo/ENVO_02500007"/>
            <rdf:Description rdf:about="http://purl.obolibrary.org/obo/ENVO_02500008"/>
            <rdf:Description rdf:about="http://purl.obolibrary.org/obo/ENVO_02500034"/>
            <rdf:Description rdf:about="http://purl.obolibrary.org/obo/RO_0000056#carbon_cycling"/>
        </owl:members>
    </rdf:Description>
</rdf:RDF>



<!-- Generated by the OWL API (version 4.2.8.20170104-2310) https://github.com/owlcs/owlapi -->

