<?xml version="1.0"?>


<!DOCTYPE rdf:RDF [
    <!ENTITY prov "http://www.w3.org/ns/prov#" >
    <!ENTITY owl  "http://www.w3.org/2002/07/owl#" >
    <!ENTITY xsd  "http://www.w3.org/2001/XMLSchema#" >
    <!ENTITY rdfs "http://www.w3.org/2000/01/rdf-schema#" >
    <!ENTITY rdf  "http://www.w3.org/1999/02/22-rdf-syntax-ns#" >
]>


<rdf:RDF xmlns="http://purl.org/provone/v1/ontology#"
     xml:base="http://purl.org/provone/v1/ontology"
     xmlns:rdfs="http://www.w3.org/2000/01/rdf-schema#"
     xmlns:prov="http://www.w3.org/ns/prov#"
     xmlns:owl="http://www.w3.org/2002/07/owl#"
     xmlns:xsd="http://www.w3.org/2001/XMLSchema#"
     xmlns:rdf="http://www.w3.org/1999/02/22-rdf-syntax-ns#">
    <owl:Ontology rdf:about="http://purl.org/provone/v1/ontology">
        <rdfs:label>DataONE PROV Extension for Scientific Workflow Provenance, Version 1</rdfs:label>
        <rdfs:seeAlso>http://www.w3.org/ns/prov</rdfs:seeAlso>
        <prov:specializationOf>http://www.w3.org/ns/prov-o</prov:specializationOf>
        <owl:versionInfo>Version 1.0</owl:versionInfo>
        <rdfs:comment>This document describes an extension of the W3C PROV standard for scientific workflow provenance.  It represents a potential standard published publicly for evaluation and possible adoption.  However, it is not associated with and is not supported by any standards organization.</rdfs:comment>
        <owl:imports rdf:resource="http://www.w3.org/ns/prov#"/>
    </owl:Ontology>
    


    <!-- 
    ///////////////////////////////////////////////////////////////////////////////////////
    //
    // Object Properties
    //
    ///////////////////////////////////////////////////////////////////////////////////////
     -->

    


    <!-- http://purl.org/provone/v1/ontology#CLtoDestP -->

    <owl:ObjectProperty rdf:about="http://purl.org/provone/v1/ontology#CLtoDestP">
        <rdfs:label>CLtoDestP</rdfs:label>
        <prov:category>Relates a SeqCtrlLink to its destination Program.</prov:category>
        <prov:category>workflow-specification</prov:category>
        <rdfs:range rdf:resource="http://purl.org/provone/v1/ontology#Program"/>
        <rdfs:domain rdf:resource="http://purl.org/provone/v1/ontology#SeqCtrlLink"/>
    </owl:ObjectProperty>
    


    <!-- http://purl.org/provone/v1/ontology#DLToInPort -->

    <owl:ObjectProperty rdf:about="http://purl.org/provone/v1/ontology#DLToInPort">
        <rdfs:label>DLToInPort</rdfs:label>
        <rdfs:comment>Connects a DataLink to an InputPort of a Program, while the same DataLink can be connected to an OutputPort of another Program.</rdfs:comment>
        <prov:category>workflow-specification</prov:category>
        <rdfs:domain rdf:resource="http://purl.org/provone/v1/ontology#DataLink"/>
        <rdfs:range rdf:resource="http://purl.org/provone/v1/ontology#InputPort"/>
    </owl:ObjectProperty>
    


    <!-- http://purl.org/provone/v1/ontology#DLToOutPort -->

    <owl:ObjectProperty rdf:about="http://purl.org/provone/v1/ontology#DLToOutPort">
        <rdfs:label>DLToOutPort</rdfs:label>
        <prov:category>workflow-specification</prov:category>
        <rdfs:comment>Connects a DataLink to the OutputPort of a Program. In turn, the same DataLink can be linked to the OutputPort of a nested Program.</rdfs:comment>
    </owl:ObjectProperty>
    


    <!-- http://purl.org/provone/v1/ontology#dataOnLink -->

    <owl:ObjectProperty rdf:about="http://purl.org/provone/v1/ontology#dataOnLink">
        <rdfs:label>dataOnLink</rdfs:label>
        <rdfs:comment>Specifies that a particular Data item was associated with a particular DataLink of a Workflow during its execution. It effectively links the trace information of a workflow to the workflow structure, by capturing the dataflow event.</rdfs:comment>
        <prov:category>trace-specification</prov:category>
        <rdfs:domain rdf:resource="http://purl.org/provone/v1/ontology#Data"/>
        <rdfs:range rdf:resource="http://purl.org/provone/v1/ontology#DataLink"/>
    </owl:ObjectProperty>
    


    <!-- http://purl.org/provone/v1/ontology#hasDefaultParam -->

    <owl:ObjectProperty rdf:about="http://purl.org/provone/v1/ontology#hasDefaultParam">
        <rdfs:label>hasDefaultParam</rdfs:label>
        <prov:category>workflow-specification</prov:category>
        <rdfs:comment>Specifies that a given InputPort has a certain Data item as a default parameter. This enables to specify especially configured Workflow instances.</rdfs:comment>
        <rdfs:range rdf:resource="http://purl.org/provone/v1/ontology#Data"/>
        <rdfs:domain rdf:resource="http://purl.org/provone/v1/ontology#InputPort"/>
    </owl:ObjectProperty>
    


    <!-- http://purl.org/provone/v1/ontology#hasInPort -->

    <owl:ObjectProperty rdf:about="http://purl.org/provone/v1/ontology#hasInPort">
        <rdfs:label>hasInPort</rdfs:label>
        <rdfs:comment>Enables to specify the InputPorts of a particular Program.</rdfs:comment>
        <prov:category>workflow-specification</prov:category>
        <rdfs:range rdf:resource="http://purl.org/provone/v1/ontology#InputPort"/>
        <rdfs:domain rdf:resource="http://purl.org/provone/v1/ontology#Program"/>
    </owl:ObjectProperty>
    


    <!-- http://purl.org/provone/v1/ontology#hasOutPort -->

    <owl:ObjectProperty rdf:about="http://purl.org/provone/v1/ontology#hasOutPort">
        <rdfs:label>hasOutPort</rdfs:label>
        <prov:category>workflow-specification</prov:category>
        <rdfs:comment>Enables to specify the OutputPorts of a particular Program.</rdfs:comment>
        <rdfs:range rdf:resource="http://purl.org/provone/v1/ontology#OutputPort"/>
        <rdfs:domain rdf:resource="http://purl.org/provone/v1/ontology#Program"/>
    </owl:ObjectProperty>
    


    <!-- http://purl.org/provone/v1/ontology#hasSubProgram -->

    <owl:ObjectProperty rdf:about="http://purl.org/provone/v1/ontology#hasSubProgram">
        <rdfs:label>hasSubProgram</rdfs:label>
        <prov:category>workflow-specification</prov:category>
        <rdfs:comment>Specifies the recursive composition of Programs, a parent Program includes a child Program as part of its specification.</rdfs:comment>
        <rdfs:domain rdf:resource="http://purl.org/provone/v1/ontology#Program"/>
        <rdfs:range rdf:resource="http://purl.org/provone/v1/ontology#Program"/>
    </owl:ObjectProperty>
    


    <!-- http://purl.org/provone/v1/ontology#inPortToDL -->

    <owl:ObjectProperty rdf:about="http://purl.org/provone/v1/ontology#inPortToDL">
        <rdfs:label>inPortToDL</rdfs:label>
        <prov:category>workflow-specification</prov:category>
        <rdfs:comment>Connects the InputPort of a Program to a DataLink. In turn, the same DataLink can then be connected to the InputPort of a nested Program.</rdfs:comment>
    </owl:ObjectProperty>
    


    <!-- http://purl.org/provone/v1/ontology#isPartOf -->

    <owl:ObjectProperty rdf:about="http://purl.org/provone/v1/ontology#isPartOf">
        <rdfs:label>isPartOf</rdfs:label>
        <prov:category>trace-specification</prov:category>
        <rdfs:comment>Specifies the structure of Execution instances, a parent Execution (associated with a Workflow) has child Executions (associated with Programs and subworkflows).</rdfs:comment>
        <rdfs:range rdf:resource="http://purl.org/provone/v1/ontology#Execution"/>
        <rdfs:domain rdf:resource="http://purl.org/provone/v1/ontology#Execution"/>
    </owl:ObjectProperty>
    


    <!-- http://purl.org/provone/v1/ontology#outPortToDL -->

    <owl:ObjectProperty rdf:about="http://purl.org/provone/v1/ontology#outPortToDL">
        <rdfs:label>outPortToDL</rdfs:label>
        <rdfs:comment>Connects an OutputPort of a Program to a DataLink, which then can be linked to an InputPort of another Program.</rdfs:comment>
        <prov:category>workflow-specification</prov:category>
        <rdfs:range rdf:resource="http://purl.org/provone/v1/ontology#DataLink"/>
        <rdfs:domain rdf:resource="http://purl.org/provone/v1/ontology#OutputPort"/>
    </owl:ObjectProperty>
    


    <!-- http://purl.org/provone/v1/ontology#sourcePToCL -->

    <owl:ObjectProperty rdf:about="http://purl.org/provone/v1/ontology#sourcePToCL">
        <rdfs:label>sourcePToCL</rdfs:label>
        <prov:category>workflow-specification</prov:category>
        <rdfs:comment>Relates a SeqCtrlLink to its source Program.</rdfs:comment>
        <rdfs:domain rdf:resource="http://purl.org/provone/v1/ontology#Program"/>
        <rdfs:range rdf:resource="http://purl.org/provone/v1/ontology#SeqCtrlLink"/>
    </owl:ObjectProperty>
    


    <!-- http://www.w3.org/ns/prov#used -->

    <rdf:Description rdf:about="&prov;used">
        <rdfs:range rdf:resource="http://purl.org/provone/v1/ontology#Data"/>
        <rdfs:domain rdf:resource="http://purl.org/provone/v1/ontology#Execution"/>
    </rdf:Description>
    


    <!-- http://www.w3.org/ns/prov#wasAssociatedWith -->

    <rdf:Description rdf:about="&prov;wasAssociatedWith">
        <rdfs:range rdf:resource="http://purl.org/provone/v1/ontology#Program"/>
        <rdfs:domain rdf:resource="http://purl.org/provone/v1/ontology#Execution"/>
    </rdf:Description>
    


    <!-- http://www.w3.org/ns/prov#wasAttributedTo -->

    <rdf:Description rdf:about="&prov;wasAttributedTo">
        <rdfs:domain rdf:resource="http://purl.org/provone/v1/ontology#Program"/>
        <rdfs:range rdf:resource="http://purl.org/provone/v1/ontology#User"/>
    </rdf:Description>
    


    <!-- http://www.w3.org/ns/prov#wasDerivedFrom -->

    <rdf:Description rdf:about="&prov;wasDerivedFrom">
        <rdfs:range rdf:resource="http://purl.org/provone/v1/ontology#Data"/>
        <rdfs:domain rdf:resource="http://purl.org/provone/v1/ontology#Data"/>
        <rdfs:domain rdf:resource="http://purl.org/provone/v1/ontology#Program"/>
        <rdfs:range rdf:resource="http://purl.org/provone/v1/ontology#Program"/>
    </rdf:Description>
    


    <!-- http://www.w3.org/ns/prov#wasGeneratedBy -->

    <rdf:Description rdf:about="&prov;wasGeneratedBy">
        <rdfs:domain rdf:resource="http://purl.org/provone/v1/ontology#Data"/>
        <rdfs:range rdf:resource="http://purl.org/provone/v1/ontology#Execution"/>
    </rdf:Description>
    


    <!-- http://www.w3.org/ns/prov#wasInformedBy -->

    <rdf:Description rdf:about="&prov;wasInformedBy">
        <rdfs:domain rdf:resource="http://purl.org/provone/v1/ontology#Execution"/>
        <rdfs:range rdf:resource="http://purl.org/provone/v1/ontology#Execution"/>
    </rdf:Description>
    


    <!-- 
    ///////////////////////////////////////////////////////////////////////////////////////
    //
    // Classes
    //
    ///////////////////////////////////////////////////////////////////////////////////////
     -->

    


    <!-- http://purl.org/provone/v1/ontology#Data -->

    <owl:Class rdf:about="http://purl.org/provone/v1/ontology#Data">
        <rdfs:label>Data</rdfs:label>
        <rdfs:subClassOf rdf:resource="&prov;Entity"/>
        <rdfs:comment>A Data item represents the basic unit of information consumed and produced by a Program. Multiple Data items may be grouped into a Collection.</rdfs:comment>
        <prov:category>data-specification</prov:category>
    </owl:Class>
    


    <!-- http://purl.org/provone/v1/ontology#DataLink -->

    <owl:Class rdf:about="http://purl.org/provone/v1/ontology#DataLink">
        <rdfs:label>DataLink</rdfs:label>
        <rdfs:subClassOf rdf:resource="&prov;Entity"/>
        <rdfs:comment>A DataLink enables to send Data items between Programs, always connecting an OutputPort from one Program to the InputPort in another Program. It is possibe for an OutputPort as well as for an InputPort to be the source or destination of multiple DataLinks, respectively.</rdfs:comment>
        <prov:category>workflow-specification</prov:category>
    </owl:Class>
    


    <!-- http://purl.org/provone/v1/ontology#InputPort -->

    <owl:Class rdf:about="http://purl.org/provone/v1/ontology#InputPort">
        <rdfs:label>InputPort</rdfs:label>
        <rdfs:subClassOf rdf:resource="&prov;Entity"/>
        <prov:category>An InputPort enables a Program to receive input Data items, which in turn may be produced by other Programs and sent through DataLinks or specified as default parameters.</prov:category>
        <prov:category>workflow-structure</prov:category>
    </owl:Class>
    


    <!-- http://purl.org/provone/v1/ontology#OutputPort -->

    <owl:Class rdf:about="http://purl.org/provone/v1/ontology#OutputPort">
        <rdfs:label>OutputPort</rdfs:label>
        <rdfs:subClassOf rdf:resource="&prov;Entity"/>
        <prov:category>workflow-specification</prov:category>
        <prov:category>An OutputPort enables a Program to produce output Data items, which may be forwarded to other Programs via DataLinks.</prov:category>
    </owl:Class>
    


    <!-- http://purl.org/provone/v1/ontology#Program -->

    <owl:Class rdf:about="http://purl.org/provone/v1/ontology#Program">
        <rdfs:label>Program</rdfs:label>
        <rdfs:subClassOf rdf:resource="&prov;Entity"/>
        <rdfs:subClassOf rdf:resource="&prov;Plan"/>
        <prov:definition>A Program represents a computational task that consumes and produces data through its input and output ports, respectively. It can be atomic or composite, the latter case represented by a possibly nested Program. It is also subject to versioning by prov:wasDerivedFrom.</prov:definition>
        <prov:category>workflow-specification</prov:category>
    </owl:Class>
    


    <!-- http://purl.org/provone/v1/ontology#Execution -->

    <owl:Class rdf:about="http://purl.org/provone/v1/ontology#Execution">
        <rdfs:label>Execution</rdfs:label>
        <rdfs:subClassOf rdf:resource="&prov;Activity"/>
        <rdfs:comment>An Execution represents the execution of a Program. If the Program in question is a Workflow, then the Execution represents a trace of its execution.</rdfs:comment>
        <prov:category>trace-specification</prov:category>
    </owl:Class>
    


    <!-- http://purl.org/provone/v1/ontology#SeqCtrlLink -->

    <owl:Class rdf:about="http://purl.org/provone/v1/ontology#SeqCtrlLink">
        <rdfs:label>SeqCtrlLink</rdfs:label>
        <rdfs:subClassOf rdf:resource="&prov;Entity"/>
        <prov:category>A SeqCtrlLink specifies a sequential control link between two Programs. A source Program is linked to a destination process, the latter can only begin its execution once the source process sends the respective signal through the link. In case a Program is the destination of multiple sequential control links, all of their activation signals must be received in order for the execution to begin.</prov:category>
        <prov:category>workflow-specification</prov:category>
    </owl:Class>
    


    <!-- http://purl.org/provone/v1/ontology#User -->

    <owl:Class rdf:about="http://purl.org/provone/v1/ontology#User">
        <rdfs:label>User</rdfs:label>
        <rdfs:subClassOf rdf:resource="&prov;Agent"/>
        <prov:category>user-specification</prov:category>
        <prov:definition>An User is the person responsible for the specification of a Program, which in turn can be a Workflow. Its specification serves attribution and accountability purposes.</prov:definition>
    </owl:Class>
    


    <!-- http://purl.org/provone/v1/ontology#Workflow -->

    <owl:Class rdf:about="http://purl.org/provone/v1/ontology#Workflow">
        <rdfs:label>Workflow</rdfs:label>
        <rdfs:subClassOf rdf:resource="http://purl.org/provone/v1/ontology#Program"/>
        <prov:category>workflow-specification</prov:category>
        <prov:definition>A Workflow is a distinguished Program, which indicates that is meant to represent the computational experiment in its entirety. It is also subject to versioning by prov:wasDerivedFrom through its super-class provone:Program.</prov:definition>
    </owl:Class>
</rdf:RDF>



<!-- Generated by the OWL API (version 3.4.2) http://owlapi.sourceforge.net -->

